unity/refinement.lean
@@ -9,13 +9,21 @@ open unity
 open temporal
 open predicate
 
-universe variables u
+universe variables u u'
 
-variables {α : Type u}
+variables {α β : Type u}
+variables {σ : Type u'}
 
 def refined (s s' : α) [system_sem α] : Prop :=
 system_sem.ex s' ⟹ system_sem.ex s
 
 infix ` ⊑ `:80 := refined
+
+def data_ref [system_sem α] [system_sem β]
+    (s : α)  (f : unity.state α  → σ)
+    (s' : β) (g : unity.state β  → σ) : Prop :=
+∀ τ : stream (unity.state β), system_sem.ex s' τ
+→ ∃ τ', system_sem.ex s τ' ∧ (g ∘ τ) = (f ∘ τ')
+
 
 end unity.refinement
