unity/models/refinement/resched_data_ref.lean
@@ -1,0 +1,216 @@
+
+import unity.temporal
+import unity.refinement
+import unity.models.nondet
+
+import util.cast
+
+namespace hidden_state
+
+universe variable u
+
+open nondet
+open temporal
+
+section defs
+
+variables {α β σ : Type}
+
+structure refined
+       (f : α → σ)
+       (ma : @prog α)
+       (g : β → σ)
+       (mc : @prog β) :=
+  (glue : α → β → Prop)
+  (obs_cons : ∀ a c, glue a c → f a = g c)
+  (bij : mc.lbl = ma.lbl)
+  (sim_init : ∀ c₀, mc^.first c₀
+            → ∃ a₀, glue a₀ c₀ ∧  ma^.first a₀)
+  (sim' : ∀ e c c' a, glue a c
+           → mc.step_of e c c'
+           → ∃ a',  ma.step_of (e.cast bij) a a'
+                  ∧ glue a' c')
+  (coarse : ∀ e a c, glue a c
+               → (  mc.coarse_sch_of e c
+                  ↔ ma.coarse_sch_of (e.cast bij) a))
+  (fine : ∀ e a c, glue a c
+               → (  mc.fine_sch_of e c
+                  ↔ ma.fine_sch_of (e.cast bij) a))
+
+end defs
+
+open unity.refinement
+
+section thm
+
+open unity
+
+parameters {α β σ : Type}
+
+parameters
+       (f : α → σ)
+       (ma : @prog α)
+       (g : β → σ)
+       (mc : @prog β)
+
+parameter R : refined f ma g mc
+
+parameter [nonempty (unity.state (@prog α))]
+parameter Tc : stream (unity.state (@prog β))
+parameter Hc : system_sem.ex mc Tc
+
+-- set_option pp.implicit true
+
+open nat
+
+noncomputable def Tevt  : stream (option (mc.lbl))
+  | i := classical.epsilon $ λ e, mc.step_of e (Tc i) (Tc (succ i))
+
+-- ∀ τ, τ ∈ Mc ⟹ ∃ τ', τ' ∈ Ma ∧ obs.τ = obs.τ'
+include Hc
+
+example (i : ℕ) : mc.step_of (Tevt i) (Tc i) (Tc $ succ i) :=
+begin
+  unfold Tevt,
+  pose P := (λ (e : option (mc.lbl)), prog.step_of mc e (Tc i) (Tc (succ i))),
+  apply @classical.epsilon_spec _ P,
+  revert P, simp,
+  note H := Hc.safety i,
+  unfold step has_safety.step is_step action stream.drop at H,
+  apply exists_imp_exists _ H,
+  intros e, simp [add_one_eq_succ],
+  apply id,
+end
+
+omit Hc
+
+noncomputable def Ta : stream (unity.state (@prog α))
+  | 0 := classical.epsilon (λ a, R.glue a (Tc 0) ∧ ma^.first a)
+  | (succ n) := classical.epsilon (λ a, R.glue a (Tc (succ n)) ∧ ma.step_of ((Tevt n).cast R.bij) (Ta n) a)
+
+include Hc
+
+lemma init_simmed
+: R.glue (Ta 0) (Tc 0) ∧ ma^.first (Ta 0) :=
+begin
+  unfold Ta,
+  apply @classical.epsilon_spec _ (λ a, R.glue a (Tc 0) ∧ ma.first a),
+  note H := Hc.init,
+  apply R.sim_init _ H,
+end
+
+include R
+
+lemma conc_step (i : ℕ)
+: mc.step_of (Tevt i) (Tc i) (Tc (succ i)) :=
+begin
+  pose P := (λ (e : option (mc.lbl)), prog.step_of mc e (Tc i) (Tc (succ i))),
+  unfold Tevt,
+  apply @classical.epsilon_spec _ P,
+  revert P, simp,
+  note H := Hc.safety i,
+  unfold temporal.action stream.drop at H,
+  simp [add_one_eq_succ] at H,
+  unfold step has_safety.step is_step at H,
+  apply exists_imp_exists _ H,
+  intro ec,
+  apply id,
+end
+
+lemma abs_step (i : ℕ) [nonempty α]
+  (J : R.glue (Ta i) (Tc i))
+:   R.glue (Ta (succ i)) (Tc (succ i))
+  ∧ ma.step_of ((Tevt i).cast R.bij) (Ta i) (Ta (succ i)) :=
+begin
+  unfold Ta,
+  pose P := (λ a, R.glue a (Tc (succ i)) ∧ ma.step_of ((Tevt _ Tc i).cast R.bij) (Ta _ _ _ _ R Tc i) a),
+  apply @classical.epsilon_spec _ P,
+  revert P, simp,
+  note H' := R.sim' (Tevt _ Tc i) _ (Tc $ succ i) (Ta _ ma _ _ R Tc i) J (conc_step _ _ _ _ R Tc Hc i),
+  apply exists_imp_exists _ H',
+  intro, apply (and_comm _ _).mp,
+end
+
+-- problem: Ta (succ i) might be chosen to satisfy a different concrete event
+-- implementable?
+
+-- we must prove []<>[cevt] ⟹ []<>[aevt] instead of [cevt] ⟹ [aevt].
+-- If cevt simulates more than one abstract event that don't agree with each other
+-- when cevt occurs, we must choose one of aevt.
+
+lemma abs_step' (i : ℕ) [nonempty α]
+  (evt : option mc.lbl)
+  (J : R.glue (Ta i) (Tc i))
+  (ACT : mc.step_of evt (Tc i) (Tc (succ i)))
+:   R.glue (Ta (succ i)) (Tc (succ i))
+  ∧ ma.step_of (evt.cast R.bij) (Ta i) (Ta (succ i)) :=
+sorry
+
+theorem glued [nonempty α] (i : ℕ) : R.glue (Ta i) (Tc i) :=
+begin
+  induction i with i,
+  { apply (init_simmed _ _ _ _ _ _ Hc).left },
+  { apply (abs_step _ _ _ _ R _ Hc i ih_1).left },
+end
+
+-- include R
+
+theorem simmed [nonempty α] (i : ℕ) : is_step ma (Ta i) (Ta (succ i)) :=
+begin
+  apply is_step_inst _ _,
+  apply (abs_step _ _ _ _ R _ Hc i _).right,
+  apply glued _ _ _ _ _ _ Hc,
+  apply_instance,
+end
+
+open unity
+
+theorem soundness [nonempty α] : data_ref ma f mc g :=
+begin
+  intros Tc Hc,
+  existsi (Ta _ ma _ mc R Tc),
+  split,
+  apply prog.ex.mk ,
+  { apply (init_simmed _ _ _ _ _ _ Hc).right },
+  { intro i,
+    unfold action step has_safety.step stream.drop,
+    simp [add_one_eq_succ],
+    apply simmed _ _ _ _ _ _ Hc,
+    apply_instance },
+  { intro ea,
+    apply imp_mono _ _ (Hc.liveness $ ea.cast' R.bij),
+    { apply iff.mp,
+      apply exists_congr, intro i,
+      apply forall_congr, intro j,
+      unfold temporal.init stream.drop,
+      pose ec := (option.cast' ea (R.bij)),
+      rw [R.coarse ec,option_cast_cast'],
+      apply glued, apply Hc },
+    apply imp_mono _ _,
+    { apply iff.mp _,
+      apply forall_congr, intro j,
+      apply exists_congr, intro i,
+      unfold temporal.init stream.drop,
+      pose ec := (option.cast' ea (R.bij)),
+      rw [R.fine ec,option_cast_cast'],
+      apply glued, apply Hc },
+    { apply forall_imp_forall, intro j,
+      apply exists_imp_exists, intro i,
+      unfold action stream.drop,
+      simp [add_one_eq_succ,add_succ],
+      generalize (j+i) k, intros k H,
+      note GLUE := glued f ma g mc R Tc Hc k,
+      note H' := (abs_step' _ _ _ _ R _ Hc _ _ GLUE H).right,
+      rw option_cast_cast' at H',
+      apply H', }, },
+  { apply funext, intro i,
+    unfold function.comp,
+    symmetry,
+    apply R.obs_cons,
+    apply glued,
+    apply Hc },
+end
+
+end thm
+
+end hidden_state
